QR/ZK.ec
@@ -4,6 +4,7 @@ require import Basics Sim1Property.
 
 import OSS.
 (* import OMZK. *)
+clone import ZKT.SequentialComposition.
 
 
 
@@ -18,18 +19,19 @@ clone import RewBasics as Rew with type sbits <- sbits.
 section.
 
 
-declare module V <: RewMaliciousVerifier{-HP}.
+declare module V <: RewMaliciousVerifier{-Hyb.HybOrcl,-Hyb.Count,-HP}.
 declare module D <: ZKDistinguisher{-HP}.
 
 
 declare axiom Sim1_run_ll : forall (V0 <: RewMaliciousVerifier), islossless V0.challenge 
   => islossless V0.summitup => islossless Sim1(V0).run.
-declare axiom D_guess_prop : equiv[ D.guess ~ D.guess : ={glob V, arg} ==> ={res} ].
 declare axiom V_summitup_ll : islossless V.summitup. 
 declare axiom V_challenge_ll : islossless V.challenge.
 declare axiom D_guess_ll : islossless D.guess.
 declare axiom P_response_ll : islossless HP.response.
 declare axiom P_commitment_ll : islossless HP.commitment.
+
+declare axiom D_guess_prop : equiv[ D.guess ~ D.guess : ={glob V, arg, glob Hyb.Count, glob Hyb.HybOrcl} ==> ={res} ].
 
 
 declare axiom rewindable_V_plus :
@@ -50,10 +52,10 @@ lemma qr_statistical_zk stat wit &m:
           `|ideal_prob - real_prob| <= 2%r * (1%r / 2%r) ^ OSS.N.
 proof.
 progress.
-apply (statistical_zk_from_sim1 HP Sim1  V D _ _ _ _ _ _ _ _ _ _ stat wit  
+apply (statistical_zk_from_sim1 HP Sim1  V D _ _ _ _ _ _ _ _ _  _ stat wit  
    &m _ );auto. apply Sim1_run_ll. apply V_summitup_ll. apply V_challenge_ll. 
 apply P_response_ll. apply P_commitment_ll.
-apply D_guess_ll. apply D_guess_prop.
+apply D_guess_ll.  apply D_guess_prop.
 apply (sim1_rew_ph V). 
  apply V_summitup_ll. apply V_challenge_ll.  apply (rewindable_A_plus V). 
 apply rewindable_V_plus.
@@ -61,11 +63,61 @@ progress.
 rewrite (sim1_prop V D _ _  _ _   ).  apply (rewindable_A_plus V).
 apply rewindable_V_plus.
 apply V_summitup_ll.
-apply V_challenge_ll. apply D_guess_ll. conseq D_guess_prop. auto. auto. auto.
+apply V_challenge_ll. apply D_guess_ll. (* conseq D_guess_prop. *) auto. auto. auto.
 progress.
-rewrite (sim1assc V D _ _ _ _  _ &m0 stat0). apply (rewindable_A_plus V).
+rewrite (sim1assc V D _ _ _ _  &m0 stat0). apply (rewindable_A_plus V).
 apply rewindable_V_plus.
 apply V_summitup_ll.
-apply V_challenge_ll. apply D_guess_ll. conseq D_guess_prop. auto. auto. 
+apply V_challenge_ll. apply D_guess_ll. (* conseq D_guess_prop. *) auto. auto. 
+
+qed.
+
+end section.
+
+
+
+section.
+
+declare module V <: RewMaliciousVerifier{-HP, -Hyb.Count, -Hyb.HybOrcl}.
+declare module D <: ZKDistinguisher{-HP, -Hyb.Count, -Hyb.HybOrcl}.
+
+
+declare axiom Sim1_run_ll : forall (V0 <: RewMaliciousVerifier), islossless V0.challenge 
+  => islossless V0.summitup => islossless Sim1(V0).run.
+declare axiom D_guess_prop : equiv[ D.guess ~ D.guess : ={glob V, arg} ==> ={res} ].
+declare axiom V_summitup_ll : islossless V.summitup. 
+declare axiom V_challenge_ll : islossless V.challenge.
+declare axiom D_guess_ll : islossless D.guess.
+declare axiom P_response_ll : islossless HP.response.
+declare axiom P_commitment_ll : islossless HP.commitment.
+
+
+lemma qr_statistical_zk_iter stat wit &m:
+        zk_relation stat wit =>
+        let real_prob = Pr[ZKRealAmp(HP, V, D).run(stat, wit) @ &m : res] in
+        let ideal_prob = Pr[ZKIdeal(SimAmp(SimN(Sim1)), V, D).run(stat, wit) @ &m : res] in
+          `|ideal_prob - real_prob| <= n%r * (2%r * (1%r / 2%r) ^ OSS.N).
+
+
+
+progress.
+apply (zk_seq HP (SimN(Sim1)) V D _ _ _ _ _ _ _ _ &m  (2%r * (1%r / 2%r) ^ OSS.N) stat wit). 
+progress. admit.
+
+admit. admit.  admit. admit. admit. 
+admit. apply D_guess_prop.
+admit.
+
+
+
+
+progress.
+
+
+apply (qr_statistical_zk V  (Di(D, SimN(Sim1),V)) _ _ _ _ _ _ _ _ stat wit &n _).
+admit. admit. admit. admit. admit.
+admit.
+proc. 
+call D_guess_prop. sim. admit. 
 auto.
 qed.
